Completed the verification of insertion sort, which required some additional lemmas about lists. Added a Hoare logic rule for local variables. Began work on quicksort.

utp/examples/insertion_sort.thy
@@ -1,89 +1,150 @@
+subsection \<open> Verification of Insertion Sort (with Local Variables) \<close>
+
 theory insertion_sort
   imports "UTP.utp" "HOL-Library.Permutation"
-begin
+begin recall_syntax
 
-alphabet st_insertion_sort =
+utp_lit_vars
+
+alphabet global =
   arr :: "int list"
+
+declare global.splits [alpha_splits del]
+
+alphabet local = global +
   i   :: nat
-  key :: int
   j   :: nat
 
-abbreviation insertion_sort :: "int list \<Rightarrow> st_insertion_sort hrel" where
+declare global.splits [alpha_splits]
+
+abbreviation lv :: "<global, _> \<Longleftrightarrow> local" where
+"lv \<equiv> \<lparr> view = (global.base\<^sub>L :: (global \<Longrightarrow> local)), coview = global.more\<^sub>L \<rparr>"
+
+lemma sym_lens_lv [simp]: "sym_lens lv"
+  by (rule sym_lens.intro, simp_all)
+
+abbreviation "I xs \<equiv> U(0 < i \<and> i < length arr \<and> j \<le> i \<and>
+      sorted(nths arr {0..<j}) \<and> sorted(nths arr {j..i}) \<and>
+      (0<j \<and> j<i  \<Rightarrow> arr!(j-1) \<le> arr!(j+1)) \<and>
+      perm arr \<guillemotleft>xs\<guillemotright>)"
+
+definition insert_elem :: "int list \<Rightarrow> local hrel" where
+"insert_elem xs =
+    while (0 < j \<and> arr!j < arr!(j-1))
+    invr @(I xs)
+    do
+      (arr[j-1], arr[j]) := (arr!j, arr!(j-1)) ;;
+      j := j - 1
+    od"
+
+abbreviation insertion_sort :: "int list \<Rightarrow> global hrel" where
   "insertion_sort xs \<equiv>
   arr := \<guillemotleft>xs\<guillemotright> ;;
-  i := 1 ;;
-  while (i < length arr) 
-  invr 
-    0 < i \<and> i < length arr \<and> sorted(nths arr {0..i-1}) \<and> perm(arr, \<guillemotleft>xs\<guillemotright>)
-  do 
-    key := arr[i] ;;
-    j := i ;;
-    while (j > 0 \<and> arr[j-1] > key)
+  open\<^bsub>lv\<^esub> ;;
+   (i := 1 ;;
+    while (i < length arr)
     invr 
-      0 < i \<and> i < length arr \<and> j \<le> i \<and> key = arr[j] \<and>
-      sorted(nths(arr, {0..<j-1})) \<and> 
-      sorted(nths(arr, {j-1..i-1})) \<and> 
-      perm(arr, \<guillemotleft>xs\<guillemotright>)
-    do
-      arr[j] := arr[j-1] ;;
-      arr[j-1] := key ;;
-      j := j - 1
-    od ;;
-    i := i + 1
-  od"
+      0 < i \<and> i \<le> length arr \<and> sorted(nths arr {0..i-1}) \<and> perm arr \<guillemotleft>xs\<guillemotright>
+    do 
+      j := i ;;
+      insert_elem xs ;;
+      i := i + 1
+    od) ;;
+  close\<^bsub>lv\<^esub>"
 
-lemma "TRY(id \<Turnstile> insertion_sort [4,3,7,1,12,8])"
-  apply (sym_eval)
-  oops
-
-lemma "{{i < #arr \<and> j \<le> i \<and> key = arr[j] \<and> sorted(nths(arr, {0..<j-1})) \<and> sorted (nths(arr, {j-1..i-1})) \<and> perm(arr, \<guillemotleft>xs\<guillemotright>)}}
-    while (j > 0 \<and> arr[j-1] > key)
-    do
-      arr[j] := arr[j-1] ;;
-      arr[j-1] := key ;;
-      j := j - 1
-    od
-    {{(\<not> (j > 0 \<and> arr[j-1] > key)) \<and> (i < #arr \<and> j \<le> i \<and> key = arr[j] \<and> sorted(nths(arr, {0..<j-1})) \<and> sorted (nths(arr, {j-1..i-1})) \<and> perm(arr, \<guillemotleft>xs\<guillemotright>))}}"
-  apply (rule while_hoare_r)
-  apply (rel_auto)
-     apply (smt Suc_diff_Suc diff_less_Suc diff_zero length_list_augment_1 length_list_augment_2 less_trans_Suc linorder_not_less nat_less_le)
-  apply (simp add: nth_list_augment)
-    apply (subst nths_list_augment_out)
-  apply (auto)
-     apply (metis diff_less_Suc length_list_augment_1 length_list_augment_2 less_imp_diff_less linorder_not_less)
-    apply (subst nths_list_augment_out)
-  apply (auto)
-    apply (metis Suc_pred diff_Suc_less le_simps(2) sorted_nths_atLeastLessThan_0)
-   defer
-   apply (simp add: list_augment_as_update)
-   apply (rename_tac arr i j)
-  apply (subgoal_tac "arr[j := arr!(j - Suc 0), j - Suc 0 := arr!j] <~~> arr")
-  apply blast
-  apply (simp add: perm_swap)
-  oops
-
-lemma "{{true}}insertion_sort xs{{arr = sort(\<guillemotleft>xs\<guillemotright>)}}"
-  apply (rule hoare_safe)
-     apply (simp_all add: unrest)
-  apply (rule hoare_safe)
-     apply (simp_all add: unrest)
-  apply (rule hoare_safe)
-    apply (rule hoare_safe) back
-       apply (simp_all add: unrest)
-    apply (rule hoare_safe) back
-       apply (simp_all add: unrest)
-    apply (rule seq_hoare_inv_r_3)
+lemma insert_elem_correct: "
+    \<lbrace>0 < i \<and> i < length arr \<and> j = i \<and> sorted(nths arr {0..i-1}) \<and> perm arr \<guillemotleft>xs\<guillemotright>\<rbrace>
+    insert_elem xs
+    \<lbrace>0 < i \<and> i < length arr \<and> sorted(nths arr {0..i}) \<and> perm arr \<guillemotleft>xs\<guillemotright>\<rbrace>\<^sub>u"
+  apply (simp add: insert_elem_def)
   apply (rule while_invr_hoare_r)
-  apply (hoare_auto)
-  apply (metis (no_types, lifting) Suc_le_eq Suc_pred diff_less_Suc length_list_augment_1 length_list_augment_2 less_le_trans not_less)
-  apply (simp_all add: nth_list_augment list_augment_as_update)
-  apply (smt Suc_le_eq Suc_le_mono Suc_pred atLeastLessThan_iff diff_diff_cancel diff_is_0_eq diff_le_self nat_less_le nths_list_update_out sorted_nths_atLeastLessThan_0)
-        defer
-        defer
-  apply (rel_auto)
-         apply (metis Suc_pred atLeast0AtMost atLeast0LessThan diff_le_self lessThan_Suc_atMost sorted_nths_atLeastLessThan_0)
-        defer
-  apply (rel_auto)
+    apply (hoare_split)
+    apply (rel_auto'; simp_all add: list_augment_as_update)
+   apply (metis diff_le_self lessThan_iff linorder_not_less nths_atLeastLessThan_0_take nths_list_update_out nths_upt_eq_take order_less_irrefl sorted_nths_atLeastLessThan_0)
+          apply (simp add: nths_uptoLessThan nths_single)
+  apply (meson diff_le_self le_less_trans perm.trans perm_swap)
+       apply (rename_tac arr i)
+  apply (smt Suc_pred diff_Suc_Suc diff_le_self diff_less diff_zero le_less_trans less_imp_le_nat nths_upt_length nths_upt_nth sorted_iff_nth_mono zero_less_Suc)
+  apply (metis One_nat_def atLeastLessThan_iff diff_le_self le_less le_less_trans less_irrefl nths_list_update_out sorted_nths_atLeastLessThan_0)
+  apply (simp add: sorted_iff_nth_mono_less nths_upt_le_length nths_upt_le_nth)
+      apply (auto)[1]
+  apply (rename_tac arr i j m n)
+     apply (case_tac "m>1")
+      apply (simp)
+      apply (drule_tac x="m-1" in spec) back
+  apply (drule_tac x="n-1" in spec) back
+      apply (simp)
+     apply (simp)
+     apply (subgoal_tac "m\<in>{0,1}")
+      apply (case_tac "n>1")
+  defer (* apply (smt Nat.add_diff_assoc2 Nat.diff_diff_right Suc_pred diff_Suc_Suc diff_commute diff_diff_cancel gr0I lessI less_nat_zero_code nat_le_linear nat_neq_iff zero_less_diff) *)
+       apply (simp)
+       apply (subgoal_tac "n=1")
+  apply (simp)
+       apply linarith
+  apply (metis One_nat_def insert_iff less_one linorder_neqE_nat)
+  apply (smt diff_le_self le_less_trans mset_eq_perm mset_swap)
+  apply (rename_tac arr i j)
+    apply (subgoal_tac " (nths arr {0..<j}) ! (j - Suc (Suc 0)) \<le> (nths arr {0..<j}) ! (j - Suc 0)")
+         apply (simp add: nths_upt_nth)
+    apply (rule sorted_nth_mono)
+            apply (simp)
+  apply linarith
+  apply (metis Suc_le_lessD Suc_pred diff_zero eq_imp_le le_less_trans less_imp_le_nat nths_upt_length)
+    apply (rel_auto')
+  apply (simp add: nths_atLeastAtMost_0_take nths_atLeastLessThan_0_take)
+  apply (simp add: nths_single)
+   apply (rel_auto')
+  using neq0_conv apply blast
+  apply (smt Suc_diff_le Suc_leI add.commute add.left_neutral atLeastLessThanSuc_atLeastAtMost diff_Suc_1 diff_Suc_less diff_is_0_eq' diff_zero le_add1 le_neq_implies_less less_imp_Suc_add less_imp_le_nat nths_upt_le_append_split nths_upt_le_nth nths_upt_length sorted_append_middle zero_less_one)
+    apply (rename_tac arr i j)
+  apply (subgoal_tac "sorted (nths arr {0..<j} @ nths arr {j..i})")
+  apply (auto)
+      apply (simp add: nths_upt_le_append_split)
+     apply (simp add: sorted_append_middle)
+  apply (auto)
+     apply (simp add: nths_upt_length nths_upt_nth nths_upt_le_nth)
+     apply (simp add: atLeast0LessThan)
+   apply (drule_tac x="0" in spec) back
+   apply (drule_tac x="n-1" in spec) back
+   apply (simp)
+  apply (subgoal_tac "arr ! Suc j \<le> arr ! (n + j - Suc 0)")
+  apply (simp)
+  apply (drule_tac x="1" in spec) back
+  apply (drule_tac x="n-1" in spec) back
+  apply (simp)
+  by (metis (no_types, lifting) Nat.add_diff_assoc Nat.add_diff_assoc2 One_nat_def Suc_lessD Suc_lessI Suc_less_eq Suc_pred le_SucI less_imp_le_nat plus_1_eq_Suc)
+
+lemma insertion_sort_correct:
+  "\<lbrace>length(xs) > 0\<rbrace>
+    insertion_sort xs
+   \<lbrace>sorted(arr) \<and> perm arr xs\<rbrace>\<^sub>u"
+  apply (rule hoare_safe) back
+     apply (simp_all add: unrest)
+  apply (rule hoare_block)
+   apply (simp)
+  apply (simp add: alpha)
+  apply (rule hoare_safe) back
+     apply (simp_all add: unrest)
+  apply (rule while_invr_hoare_r)
+  apply (rule hoare_safe) back back
+       apply (simp_all add: unrest)
+  apply (rule hoare_safe) back
+    apply (rule hoare_r_conseq)
+       apply (rule insert_elem_correct)
+      apply (rel_auto')
+    apply (rel_auto')
+      apply (rel_auto')
+  apply (simp add: Suc_leI)
+    apply (simp add: nths_single)
+      apply (rel_auto')
+   apply (simp add: nths_atLeastAtMost_0_take)
+  done
+
+lemma "TRY(id\<^sub>s \<Turnstile> insertion_sort [4,3,7,1,12,8])"
+  apply (unfold insert_elem_def)
+  apply (sym_eval)
+  apply (simp add: usubst unrest)
   oops
 
 end
