utp/examples/quicksort.thy
@@ -1,0 +1,78 @@
+subsection \<open> Quicksort \<close>
+
+theory quicksort
+  imports "UTP.utp"
+begin
+
+declare length_list_augment_2 [simp]
+
+abbreviation rforloop :: "('a::{ord,plus,one} \<Longrightarrow> 's) \<Rightarrow> ('a, 's) uexpr \<Rightarrow> ('a, 's) uexpr \<Rightarrow> 's hrel \<Rightarrow> 's hrel" 
+  ("for _ := _ to _ do _ od") 
+  where "rforloop x i j P \<equiv> x := i ;; while &x \<le> j do P ;; x := &x + 1 od"
+
+abbreviation rforloop_inv :: "('a::{ord,plus,one} \<Longrightarrow> 's) \<Rightarrow> ('a, 's) uexpr \<Rightarrow> ('a, 's) uexpr \<Rightarrow> 's upred \<Rightarrow> 's hrel \<Rightarrow> 's hrel" 
+  ("for _ := _ to _ invr _ do _ od")
+  where "rforloop_inv x i j I P \<equiv> x := i ;; while &x \<le> j invr I do P ;; x := &x + 1 od"
+
+utp_lift_notation rforloop (1 2)
+
+utp_lift_notation rforloop_inv (1 2 3)
+
+utp_lit_vars
+
+alphabet global = 
+  A :: "int list"
+  pivot :: int
+  i :: nat
+  j :: nat
+
+(*
+alphabet local = global +
+  pivot :: int
+  i :: nat
+  j :: nat
+
+abbreviation lv :: "<global, _> \<Longleftrightarrow> local" where
+"lv \<equiv> \<lparr> view = (global.base\<^sub>L :: (global \<Longrightarrow> local)), coview = global.more\<^sub>L \<rparr>"
+
+lemma sym_lens_lv [simp]: "sym_lens lv"
+  by (rule sym_lens.intro, simp_all)
+*)
+
+abbreviation "partition_inv p r \<equiv> 
+             U(i < j \<and> j \<le> p \<and> p \<le> r \<and> r < length A \<and> (\<forall> k. k < length A \<Rightarrow> 
+               (p \<le> k \<and> k \<le> i \<Rightarrow> A!k \<le> pivot)
+             \<and> (i + 1 \<le> k \<and> k \<le> j - 1 \<Rightarrow> pivot < A!k) 
+             \<and> (k = r \<Rightarrow> A!k = pivot)))"
+
+abbreviation partition :: "nat \<Rightarrow> nat \<Rightarrow> global hrel" where
+"partition p r \<equiv>
+   pivot := A!r ;;
+   i := (p - 1) ;;
+   for j := p to r - 1
+   invr @(partition_inv p r)
+   do
+     if (A ! j) \<le> pivot then
+       i := i + 1 ;;
+       (A[j], A[i]) := (A!i, A!j)
+     fi
+   od ;;
+   (A[i+1], A[r]) := (A!r, A!i+1)"
+
+lemma "\<lbrace>@(partition_inv p r)\<rbrace>   
+   while j \<le> r - 1
+   invr @(partition_inv p r)
+   do
+     if (A ! j) \<le> pivot then
+       i := i + 1 ;;
+       (A[j], A[i]) := (A!i, A!j)
+     fi ;;
+     j := j + 1
+   od
+   \<lbrace>@(partition_inv p r)\<rbrace>\<^sub>u"
+  apply (rule while_invr_hoare_r)
+    apply (hoare_split)
+      apply (rel_auto')
+  oops
+
+end
